<?xml version="1.0" encoding="UTF-8"?>

<!DOCTYPE rdf:RDF [
  <!ENTITY ratio  "http://sweet.jpl.nasa.gov/2.3/propDimensionlessRatio.owl#">
  <!ENTITY units  "http://sweet.jpl.nasa.gov/2.3/reprSciUnits.owl">
  <!ENTITY mrela "http://sweet.jpl.nasa.gov/2.3/relaMath.owl">
  <!ENTITY mrela2 "http://sweet.jpl.nasa.gov/2.3/relaMath.owl#">
  <!ENTITY mstat "http://sweet.jpl.nasa.gov/2.3/reprMathStatistics.owl">
  <!ENTITY screla "http://sweet.jpl.nasa.gov/2.3/relaSci.owl">
  <!ENTITY prop "http://sweet.jpl.nasa.gov/2.3/prop.owl">
  <!ENTITY quan "http://sweet.jpl.nasa.gov/2.3/propQuantity.owl">
  <!ENTITY ener "http://sweet.jpl.nasa.gov/2.3/propEnergy.owl">
  <!ENTITY spac "http://sweet.jpl.nasa.gov/2.3/propSpace.owl">
  <!ENTITY mass "http://sweet.jpl.nasa.gov/2.3/propMass.owl">
  <!ENTITY oper "http://sweet.jpl.nasa.gov/2.3/reprMathOperation.owl">
  <!ENTITY owl "http://www.w3.org/2002/07/owl#">
  <!ENTITY rdf "http://www.w3.org/1999/02/22-rdf-syntax-ns#">
  <!ENTITY rdfs "http://www.w3.org/2000/01/rdf-schema#">
  <!ENTITY xsd "http://www.w3.org/2001/XMLSchema#">
]>

<rdf:RDF xml:base="&ratio;"
         xmlns:ratio="&ratio;"
         xmlns:units="&units;"
         xmlns:mstat="&mstat;"
         xmlns:mrela="&mrela;"
         xmlns:mrela2="&mrela2;"
         xmlns:screla="&screla;"
         xmlns:spac="&spac;"
         xmlns:mass="&mass;"
         xmlns:ener="&ener;"
         xmlns:quan="&quan;"
         xmlns:oper="&oper;"
         xmlns:prop="&prop;"
         xmlns:owl="&owl;"
         xmlns:rdf="&rdf;"
         xmlns:rdfs="&rdfs;"
 	 xmlns:xsd="&xsd;">

<!-- Ontology Information -->
  <owl:Ontology rdf:about="" owl:versionInfo="2.3">
     <rdfs:label>SWEET Ontology</rdfs:label>
     <owl:imports rdf:resource="&mrela;"/>
     <owl:imports rdf:resource="&mstat;"/>
     <owl:imports rdf:resource="&screla;"/>
     <owl:imports rdf:resource="&oper;"/>
     <owl:imports rdf:resource="&mass;"/>
     <owl:imports rdf:resource="&prop;"/>
     <owl:imports rdf:resource="&ener;"/>
     <owl:imports rdf:resource="&spac;"/>
     <owl:imports rdf:resource="&quan;"/>
  </owl:Ontology>

<!-- Dimensionless ratios -->
  <owl:Class rdf:about="#DimensionlessRatio">
    <rdfs:subClassOf rdf:resource="&oper;#Ratio" />
    <rdfs:subClassOf>
      <owl:Restriction>
        <owl:hasValue rdf:resource="&units;#dimensionlessUnit"/>
        <owl:onProperty rdf:resource="&screla;#hasDefaultUnit"/>
      </owl:Restriction>
    </rdfs:subClassOf>
  </owl:Class>

  <ratio:DimensionlessRatio rdf:about="#RossbyNumber">
    <rdf:type rdf:resource="#DimensionlessRatio" />
    <rdfs:comment xml:lang="en">A dimensionless number relating the ratio of inertial to Coriolis forces for a given flow of a rotating fluid.</rdfs:comment>
  </ratio:DimensionlessRatio>

  <ratio:DimensionlessRatio rdf:about="#FroudeNumber">
  </ratio:DimensionlessRatio>

  <ratio:DimensionlessRatio rdf:about="#BulkRichardsonNumber">
    <mrela2:approximates rdf:resource="#RichardsonNumber" />
    <rdfs:comment xml:lang="en">An approximation to the gradient Richardson number formed by approximating local gradients by finite difference across layers.</rdfs:comment>
  </ratio:DimensionlessRatio>

  <ratio:DimensionlessRatio rdf:about="#CriticalRichardsonNumber">
    <mrela2:hasThreshold rdf:resource="#RichardsonNumber" />
  </ratio:DimensionlessRatio>

  <ratio:DimensionlessRatio rdf:about="#GradientRichardsonNumber">
  </ratio:DimensionlessRatio>

  <ratio:DimensionlessRatio rdf:about="#ReynoldsNumber">
    <rdf:type rdf:resource="&prop;#FluidProperty"/>
  <rdfs:comment xml:lang="en">The dimensionless ratio of the inertial force (∼U2/L) to the viscous force (∼ νU/L2) in the Navier–Stokes equations, where U is a characteristic velocity, L is a characteristic length, and ν is the kinematic viscosity of the fluid; thus, Re=ULv. The Reynolds number is of great importance in the theory of hydrodynamic stability and the origin of turbulence. The inertia force generates vortex stretching and nonlinear interactions and hence creates randomness. Turbulence occurs when the inertia term dominates the viscous term, that is, when the Reynolds number is large. For many engineering flows, turbulence occurs when Re > Rec, where the critical Reynolds number is roughly Rec = 2100.</rdfs:comment>
  </ratio:DimensionlessRatio>

  <ratio:DimensionlessRatio rdf:about="#RichardsonNumber">
  </ratio:DimensionlessRatio>

  <ratio:DimensionlessRatio rdf:about="#SonicMachNumber">
    <rdf:type rdf:resource="&prop;#MotionProperty"/>
  </ratio:DimensionlessRatio>

  <ratio:DimensionlessRatio rdf:about="#DragCoefficient">
    <rdf:type rdf:resource="&prop;#FluidProperty"/>
  </ratio:DimensionlessRatio>

 <ratio:DimensionlessRatio rdf:about="#WaterCirculationCoefficient">
    <rdfs:comment xml:lang="en">The ratio of a region's total precipitation to its external precipitation originating as evaporation from the oceans as opposed to evapotranspiration from the land. </rdfs:comment>
  </ratio:DimensionlessRatio>

  <ratio:DimensionlessRatio rdf:about="#LeafAreaIndex">
  </ratio:DimensionlessRatio>

  <ratio:DimensionlessRatio rdf:about="#RetardationFactor">
    <rdf:type rdf:resource="&prop;#HydrogeologicalProperty"/>
  <rdfs:comment xml:lang="en">The ratio of the average linear velocity of groundwater to the velocity of the retarded constituent at C/Co=0.5.</rdfs:comment>
  </ratio:DimensionlessRatio>

  <ratio:DimensionlessRatio rdf:about="#SpecificRetention">
  <rdfs:comment xml:lang="en">The ratio of the Volume of water which the porous medium, after being saturated, will retain against the pull of gravity to the volume of the porous medium.</rdfs:comment>
  </ratio:DimensionlessRatio>

  <ratio:DimensionlessRatio rdf:about="#SpecificStorage">
  <rdfs:comment xml:lang="en">The volume of water released from or taken into storage per unit volume of the porous medium per unit change in head.</rdfs:comment>
  </ratio:DimensionlessRatio>

  <ratio:DimensionlessRatio rdf:about="#SpecificYield">
  <rdfs:comment xml:lang="en">The ratio of the volume of water which the porous medium after being saturated, will yield by gravity to the volume of the porous medium.</rdfs:comment>
  </ratio:DimensionlessRatio>

  <ratio:DimensionlessRatio rdf:about="#AngstromExponent">
    <rdf:type rdf:resource="&quan;#RadiationMediumInteractionQuantity"/>
  </ratio:DimensionlessRatio>

  <ratio:DimensionlessRatio rdf:about="#VonKarmanConstant">
    <rdf:type rdf:resource="&quan;#PhysicalConstant" />
  </ratio:DimensionlessRatio>

  <ratio:DimensionlessRatio rdf:about="#RelativePermeability">
  <rdfs:comment xml:lang="en"> The ratio of the effective permeability for a given flow phase to the intrinsic permeability of the porous medium (WMO, 1974). The ratio of the effective and specific permeabilities.</rdfs:comment>
  </ratio:DimensionlessRatio>

  <ratio:DimensionlessRatio rdf:about="#PecletNumber">
    <rdfs:comment>A relationship between the advective and diffusive components of solute transport expressed as the ratio of the product of the average interstitial velocity, times the characteristic length, divided by the coefficient of molecular diffusion; small values indicate diffusion dominance, large values indicate advection dominance.</rdfs:comment>
  </ratio:DimensionlessRatio>

  <ratio:DimensionlessRatio rdf:about="#RouseNumber">
  </ratio:DimensionlessRatio>

  <ratio:DimensionlessRatio rdf:about="#SignalToNoiseRatio">
  </ratio:DimensionlessRatio>

  <owl:Class rdf:about="#BowenRatio">
    <rdfs:subClassOf rdf:resource="&oper;#Ratio" />
    <rdfs:subClassOf>
      <owl:Restriction>
        <owl:allValuesFrom rdf:resource="&ener;#SensibleHeat"/>
        <owl:onProperty rdf:resource="&mrela;#hasFirstOperand"/>
      </owl:Restriction>
    </rdfs:subClassOf>
    <rdfs:subClassOf>
      <owl:Restriction>
        <owl:allValuesFrom rdf:resource="&ener;#LatentHeat"/>
        <owl:onProperty rdf:resource="&mrela;#hasSecondOperand"/>
      </owl:Restriction>
    </rdfs:subClassOf>
  </owl:Class>

  <ratio:DimensionlessRatio rdf:about="#DepolarizationRatio">
    <rdfs:comment xml:lang="en">In Raman spectroscopy, the depolarization ratio is the intensity ratio between the perpendicular component and the parallel component of the Raman scattered light.</rdfs:comment>
  </ratio:DimensionlessRatio>

  <ratio:DimensionlessRatio rdf:about="#IsotopeRatio">
  </ratio:DimensionlessRatio>

  <ratio:DimensionlessRatio rdf:about="#AspectRatio">
   <rdf:type rdf:resource="&spac;#Shape"/>
  </ratio:DimensionlessRatio>

  <ratio:DimensionlessRatio rdf:about="#Electronegativity">
    <rdf:type rdf:resource="&quan;#ElectromagneticQuantity"/>
  </ratio:DimensionlessRatio>

  <ratio:DimensionlessRatio rdf:about="#PlasmaParameter">
    <rdf:type rdf:resource="&quan;#ElectromagneticQuantity"/>
  </ratio:DimensionlessRatio>

  <ratio:DimensionlessRatio rdf:about="#RefractiveIndex">
    <rdf:type rdf:resource="&quan;#ElectromagneticQuantity"/>
  </ratio:DimensionlessRatio>

  <ratio:DimensionlessRatio rdf:about="#HydraulicGradient">
    <rdf:type rdf:resource="&prop;#HydrogeologicalProperty"/>
    <owl:sameAs rdf:resource="#DarcySlope"/>
  </ratio:DimensionlessRatio>
  <ratio:DimensionlessRatio rdf:about="#DarcySlope"/>

  <ratio:DimensionlessRatio rdf:about="#VoidRatio">
    <rdf:type rdf:resource="&mass;#ConsistenceProperty"/>
  </ratio:DimensionlessRatio>

<!-- statistical scores -->
  <owl:Class rdf:about="#StatisticalScore">
    <rdfs:subClassOf rdf:resource="&prop;#StatisticalSummary"/>
  </owl:Class>

  <owl:Class rdf:about="#ChiSquareValue">
    <rdfs:subClassOf rdf:resource="#StatisticalScore"/>
  </owl:Class>

  <owl:Class rdf:about="#ReducedChiSquareValue">
    <rdfs:subClassOf rdf:resource="#ChiSquareValue"/>
  </owl:Class>

  <owl:Class rdf:about="#ZScore">
    <rdfs:subClassOf rdf:resource="#StatisticalScore"/>
    <rdfs:subClassOf>
      <owl:Restriction>
        <owl:allValuesFrom rdf:resource="&mstat;#ZTest"/>
        <owl:onProperty rdf:resource="&mrela;#hasTest"/>
      </owl:Restriction>
    </rdfs:subClassOf>
  </owl:Class>

  <owl:Class rdf:about="#tScore">
    <rdfs:subClassOf rdf:resource="#StatisticalScore"/>
    <rdfs:subClassOf>
      <owl:Restriction>
        <owl:allValuesFrom rdf:resource="&mstat;#tTest"/>
        <owl:onProperty rdf:resource="&mrela;#hasTest"/>
      </owl:Restriction>
    </rdfs:subClassOf>
  </owl:Class>

</rdf:RDF>
