<?xml version="1.0" encoding="UTF-8"?>

<!DOCTYPE rdf:RDF [
  <!ENTITY planet "http://sweet.jpl.nasa.gov/2.3/realm.owl#">
  <!ENTITY rela "http://sweet.jpl.nasa.gov/2.3/rela.owl#">
  <!ENTITY crela "http://sweet.jpl.nasa.gov/2.3/relaClimate.owl#">
  <!ENTITY mrela "http://sweet.jpl.nasa.gov/2.3/relaMath.owl#">
  <!ENTITY srela "http://sweet.jpl.nasa.gov/2.3/relaSci.owl#">
  <!ENTITY sreg "http://sweet.jpl.nasa.gov/2.3/realmRegion.owl#">
  <!ENTITY climate "http://sweet.jpl.nasa.gov/2.3/phenPlanetClimate.owl#">
  <!ENTITY thic "http://sweet.jpl.nasa.gov/2.3/propSpaceThickness.owl#">
  <!ENTITY zone "http://sweet.jpl.nasa.gov/2.3/realmClimateZone.owl#">
  <!ENTITY time "http://sweet.jpl.nasa.gov/2.3/reprTimeSeason.owl#">
  <!ENTITY ptime "http://sweet.jpl.nasa.gov/2.3/propTime.owl#">
  <!ENTITY math "http://sweet.jpl.nasa.gov/2.3/reprMath.owl#">
  <!ENTITY cate "http://sweet.jpl.nasa.gov/2.3/propCategorical.owl#">
  <!ENTITY temp "http://sweet.jpl.nasa.gov/2.3/propTemperature.owl#">
  <!ENTITY owl "http://www.w3.org/2002/07/owl#">
  <!ENTITY rdf "http://www.w3.org/1999/02/22-rdf-syntax-ns#">
  <!ENTITY rdfs "http://www.w3.org/2000/01/rdf-schema#">
  <!ENTITY xsd "http://www.w3.org/2001/XMLSchema#">
]>

<rdf:RDF xml:base="&zone;"
         xmlns:planet="&planet;"
         xmlns:climate="&climate;"
         xmlns:time="&time;"
         xmlns:ptime="&ptime;"
         xmlns:math="&math;"
         xmlns:temp="&temp;"
         xmlns:thic="&thic;"
         xmlns:cate="&cate;"
         xmlns:rela="&rela;"
         xmlns:crela="&crela;"
         xmlns:mrela="&mrela;"
         xmlns:srela="&srela;"
         xmlns:sreg="&sreg;"
         xmlns:zone="&zone;"
         xmlns:owl="&owl;"
         xmlns:rdf="&rdf;"
         xmlns:rdfs="&rdfs;"
	 xmlns:xsd = "&xsd;">

<!-- Ontology Information -->
  <owl:Ontology rdf:about=""
                owl:versionInfo="2.3">
     <rdfs:label>SWEET Ontology</rdfs:label>
     <owl:imports rdf:resource="http://sweet.jpl.nasa.gov/2.3/reprTimeSeason.owl"/>
     <owl:imports rdf:resource="http://sweet.jpl.nasa.gov/2.3/propTime.owl"/>
     <owl:imports rdf:resource="http://sweet.jpl.nasa.gov/2.3/reprMath.owl"/>
     <owl:imports rdf:resource="http://sweet.jpl.nasa.gov/2.3/propTemperature.owl"/>
     <owl:imports rdf:resource="http://sweet.jpl.nasa.gov/2.3/realmRegion.owl"/>
     <owl:imports rdf:resource="http://sweet.jpl.nasa.gov/2.3/realm.owl"/>
     <owl:imports rdf:resource="http://sweet.jpl.nasa.gov/2.3/rela.owl"/>
     <owl:imports rdf:resource="http://sweet.jpl.nasa.gov/2.3/relaClimate.owl"/>
     <owl:imports rdf:resource="http://sweet.jpl.nasa.gov/2.3/relaMath.owl"/>
     <owl:imports rdf:resource="http://sweet.jpl.nasa.gov/2.3/relaSci.owl"/>
     <owl:imports rdf:resource="http://sweet.jpl.nasa.gov/2.3/propCategorical.owl"/>
     <owl:imports rdf:resource="http://sweet.jpl.nasa.gov/2.3/phenPlanetClimate.owl"/>
  </owl:Ontology>

<!-- Annotation Properties -->
  <owl:AnnotationProperty rdf:about="&owl;versionInfo"/>

<!-- Climate Zone Types -->

  <owl:Class rdf:ID="ClimateClassification">
    <rdfs:subClassOf rdf:resource="&cate;Category"/>
  </owl:Class>

  <owl:Class rdf:about="#ClimateZoneType">
    <rdfs:subClassOf rdf:resource="#ClimateClassification"/>
  </owl:Class>

  <owl:Class rdf:about="#MarineClimate">
    <rdfs:subClassOf rdf:resource="#ClimateClassification" />
    <rdfs:subClassOf>
      <owl:Restriction>
        <owl:onProperty rdf:resource="&rela;hasRealm" />
        <owl:someValuesFrom rdf:resource="&planet;Ocean" />
      </owl:Restriction>
    </rdfs:subClassOf>
    <rdfs:comment xml:lang="en">(Also called maritime climate, oceanic climate.) A regional climate under the predominant influence of the sea, characterized by relatively small seasonal variations and high atmospheric moisture content; the antithesis of a continental climate.</rdfs:comment>
  </owl:Class>

  <owl:Class rdf:about="#RainShadow">
    <rdfs:subClassOf rdf:resource="#ClimateZoneType"/>
    <rdfs:comment xml:lang="en">A region of sharply reduced precipitation on the lee side of an orographic barrier, as compared with regions upwind of the barrier.</rdfs:comment>
  </owl:Class>

  <owl:Class rdf:about="#Doldrums">
    <rdfs:subClassOf rdf:resource="#ClimateZoneType"/>
    <rdfs:subClassOf>
      <owl:Restriction>
        <owl:onProperty rdf:resource="&rela;hasRealm" />
        <owl:hasValue rdf:resource="&sreg;LowLatitude" />
        </owl:Restriction>
    </rdfs:subClassOf>
    <rdfs:comment xml:lang="en">A nautical term for the equatorial trough, with special reference to the light and variable nature of the winds.</rdfs:comment>
  </owl:Class>

  <owl:Class rdf:about="#DesertClimateZone">
    <rdfs:subClassOf rdf:resource="#ClimateZoneType"/>
  </owl:Class>

  <owl:Class rdf:about="#IntertropicalConvergenceZone">
    <rdfs:subClassOf rdf:resource="#ClimateZoneType"/>
    <owl:equivalentClass rdf:resource="#ITCZ"/>
    <rdfs:subClassOf>
      <owl:Restriction>
        <owl:onProperty rdf:resource="&rela;hasRealm" />
        <owl:allValuesFrom rdf:resource="#Equator" />
        </owl:Restriction>
    </rdfs:subClassOf>
  </owl:Class>
  <owl:Class rdf:about="#ITCZ"/>

  <owl:Class rdf:about="#SubtropicalClimateZone">
    <rdfs:subClassOf rdf:resource="#ClimateZoneType"/>
  </owl:Class>

  <owl:Class rdf:about="#TropicalClimateZone">
    <rdfs:subClassOf rdf:resource="#ClimateZoneType"/>
  </owl:Class>

  <owl:Class rdf:ID="DryWinterClimate">
    <rdfs:subClassOf rdf:resource="#ClimateClassification"/>
    <rdfs:subClassOf>
      <owl:Restriction>
        <owl:onProperty rdf:resource="&crela;hasDrySeason"/>
        <owl:hasValue rdf:resource="&time;Winter"/>
      </owl:Restriction>
    </rdfs:subClassOf>
  </owl:Class>

  <owl:Class rdf:ID="WetSummerClimate">
    <rdfs:subClassOf rdf:resource="#ClimateClassification"/>
    <rdfs:subClassOf>
      <owl:Restriction>
        <owl:onProperty rdf:resource="&crela;hasWetSeason"/>
        <owl:hasValue rdf:resource="&time;Summer"/>
      </owl:Restriction>
    </rdfs:subClassOf>
  </owl:Class>

  <owl:Class rdf:ID="WetSummerDryWinterClimate">
    <rdfs:subClassOf rdf:resource="#DryWinterClimate"/>
    <rdfs:subClassOf rdf:resource="#WetSummerClimate"/>
  </owl:Class>

<!-- Climate zones -->
  <owl:Class rdf:ID="A">
    <owl:equivalentClass rdf:resource="#TropicalClimate"/>
    <rdfs:subClassOf rdf:resource="#ClimateClassification"/>
    <rdfs:comment xml:lang="en">The A climate classification, also known as the Tropical climate classification, is characterized as being consistently warm with all months averaging above 18 degrees C and having annual precipitation exceeds potential evapotranspiration (POTET).</rdfs:comment>
    <rdfs:subClassOf>
      <owl:Restriction>
        <owl:onProperty rdf:resource="&crela;hasAverageAnnualPrecipitation"/>
        <owl:hasValue>
          <thic:PrecipitationRange>
            <srela:hasLowerQuantity rdf:resource="&thic;AnnualPotentialEvapotranspiration"/>
          </thic:PrecipitationRange>
        </owl:hasValue>
      </owl:Restriction>
    </rdfs:subClassOf>
    <rdfs:subClassOf>
      <owl:Restriction>
        <owl:onProperty rdf:resource="&crela;hasAverageMonthlyTemperature"/>
        <owl:hasValue>
          <temp:TemperatureRange>
            <mrela:hasLowerBound rdf:datatype="&xsd;integer">18</mrela:hasLowerBound>
          </temp:TemperatureRange>
        </owl:hasValue>
      </owl:Restriction>
    </rdfs:subClassOf>
  </owl:Class>
  <owl:Class rdf:ID="TropicalClimate"/>

  <owl:Class rdf:ID="B">
    <owl:equivalentClass rdf:resource="#DryClimate"/>
    <rdfs:subClassOf rdf:resource="#ClimateClassification"/>
    <rdfs:comment xml:lang="en">Potential evapotranspiration (POTET) exceeds precipitation in all B climates. Subdivisions are based on precipitation timing and amount and mean annual temperature.</rdfs:comment>
    <rdfs:subClassOf>
      <owl:Restriction>
        <owl:onProperty rdf:resource="&crela;hasAverageAnnualPrecipitation"/>
        <owl:hasValue>
          <thic:PrecipitationRange>
            <srela:hasLowerQuantity rdf:resource="&thic;AnnualPotentialEvapotranspiration"/>
          </thic:PrecipitationRange>
        </owl:hasValue>
      </owl:Restriction>
    </rdfs:subClassOf>
  </owl:Class>
  <owl:Class rdf:ID="DryClimate"/>

  <owl:Class rdf:ID="C">
    <rdfs:subClassOf rdf:resource="#ClimateClassification"/>
    <owl:equivalentClass rdf:resource="#TemperateClimate"/>
    <rdfs:subClassOf>
      <owl:Restriction>
        <owl:onProperty rdf:resource="&crela;hasAverageColdestMonthTemperature"/>
        <owl:hasValue>
          <temp:TemperatureRange>
            <mrela:hasLowerBound rdf:datatype="&xsd;integer">0</mrela:hasLowerBound>
            <mrela:hasUpperBound rdf:datatype="&xsd;integer">18</mrela:hasUpperBound>
          </temp:TemperatureRange>
        </owl:hasValue>
      </owl:Restriction>
    </rdfs:subClassOf>
    <rdfs:subClassOf>
      <owl:Restriction>
        <owl:onProperty rdf:resource="&crela;hasAverageWarmestMonthTemperature"/>
        <owl:hasValue>
          <temp:TemperatureRange>
            <mrela:hasLowerBound rdf:datatype="&xsd;integer">10</mrela:hasLowerBound>
            <mrela:hasUpperBound rdf:datatype="&xsd;integer">22</mrela:hasUpperBound>
          </temp:TemperatureRange>
        </owl:hasValue>
      </owl:Restriction>
    </rdfs:subClassOf>
  </owl:Class>
  <owl:Class rdf:ID="TemperateClimate"/>

  <owl:Class rdf:ID="D">
    <rdfs:subClassOf rdf:resource="#ClimateClassification"/>
    <rdfs:subClassOf>
      <owl:Restriction>
        <owl:onProperty rdf:resource="&crela;hasAverageColdestMonthTemperature"/>
        <owl:hasValue>
          <temp:TemperatureRange>
            <mrela:hasUpperBound rdf:datatype="&xsd;integer">0</mrela:hasUpperBound>
          </temp:TemperatureRange>
        </owl:hasValue>
      </owl:Restriction>
    </rdfs:subClassOf>
    <rdfs:subClassOf>
      <owl:Restriction>
        <owl:onProperty rdf:resource="&crela;hasAverageWarmestMonthTemperature"/>
        <owl:hasValue>
          <temp:TemperatureRange>
            <mrela:hasLowerBound rdf:datatype="&xsd;integer">10</mrela:hasLowerBound>
          </temp:TemperatureRange>
        </owl:hasValue>
      </owl:Restriction>
    </rdfs:subClassOf>
    <rdfs:comment xml:lang="en">The D climate classification, also known as the microthermal climate classification,  is characterized by by having the warmest month of the year above 10 degree C and the coldest below 0 degree C.</rdfs:comment>
  </owl:Class>

  <owl:Class rdf:ID="E">
    <rdfs:subClassOf rdf:resource="#ClimateClassification"/>
  </owl:Class>

<!-- Individuals -->
  <zone:A rdf:ID="Af">
    <owl:sameAs rdf:resource="#TropicalRainForestClimate"/>
    <crela:hasAverageMonthlyPrecipitation>
      <thic:PrecipitationRange_cm>
        <mrela:hasLowerBound rdf:datatype="&xsd;integer">6</mrela:hasLowerBound>
      </thic:PrecipitationRange_cm>
    </crela:hasAverageMonthlyPrecipitation>
    <rdfs:comment xml:lang="en">The Af climate classification, also known as the tropical rain forest climate classification, is characterized by monthly precipitation in excess of 6 cm all months out of year.</rdfs:comment>
  </zone:A>
  <zone:A rdf:ID="TropicalRainForestClimate"/>

  <zone:A rdf:ID="Am">
    <owl:sameAs rdf:resource="#TropicalMonsoonClimate"/>
    <crela:hasAverageDrySeasonPrecipitation>
      <thic:PrecipitationRange_cm>
        <mrela:hasUpperBound rdf:datatype="&xsd;integer">6</mrela:hasUpperBound>
      </thic:PrecipitationRange_cm>
    </crela:hasAverageDrySeasonPrecipitation>
    <crela:hasAverageITCZDominanceDuration>
      <ptime:MonthRange>
        <mrela:hasLowerBound rdf:datatype="&xsd;integer">6</mrela:hasLowerBound>
      </ptime:MonthRange>
    </crela:hasAverageITCZDominanceDuration>
    <rdfs:comment xml:lang="en">The Am climate classification, also known as Tropical Monsoon Climate, is characterized by a short marked dry season with 1 or more months receiving less than 6 cm of precipitation, an otherwise excessively wet rainy season, and ITCZ dominance for 6 - 12 months out of the year.</rdfs:comment>
  </zone:A>
  <zone:A rdf:ID="TropicalMonsoonClimate"/>

  <zone:A rdf:ID="Aw">
    <owl:sameAs rdf:resource="#TropicalSavannaClimate"/>
    <rdf:type rdf:resource="#WetSummerDryWinterClimate"/>
    <crela:hasAverageITCZDominanceDuration>
      <ptime:MonthRange>
        <mrela:hasUpperBound rdf:datatype="&xsd;integer">6</mrela:hasUpperBound>
      </ptime:MonthRange>
    </crela:hasAverageITCZDominanceDuration>
    <rdfs:comment xml:lang="en">The Aw climate classification, also known as Tropical Savanna climate classification, is characterized by a summer wet season, winter dry season, and ITCZ dominance for 6 months or less.</rdfs:comment>
  </zone:A>
  <zone:A rdf:ID="TropicalSavannaClimate"/>

  <zone:B rdf:ID="BS">
    <owl:sameAs rdf:resource="#SemiAridClimate"/>
        <crela:hasAverageAnnualPrecipitation>
          <thic:PrecipitationRange>
            <srela:hasLowerQuantity rdf:resource="&thic;AnnualHalfPotentialEvapotranspiration"/>
            <srela:hasUpperQuantity rdf:resource="&thic;AnnualPotentialEvapotranspiration"/>
          </thic:PrecipitationRange>
        </crela:hasAverageAnnualPrecipitation>
    <rdfs:comment xml:lang="en">The BS climate classification, also known as semiarid climate classification, is characterized by having precipitation amounts greater than 1/2 potential evapotranspiration (POTET), but not equal to it.</rdfs:comment>
  </zone:B>
  <zone:B rdf:ID="SemiAridClimate"/>

  <zone:B rdf:ID="BSh">
    <owl:sameAs rdf:resource="#HotLowLatitudeSteppeClimate"/>
    <rdfs:comment xml:lang="en">The BSh climate classification, also known as the hot low-latitude steppe, is characterized by having mean annual temperatures greater than 18 degree C.</rdfs:comment>
    <crela:hasAverageAnnualTemperature>
      <temp:TemperatureRange>
        <mrela:hasLowerBound rdf:datatype="&xsd;integer">18</mrela:hasLowerBound>
      </temp:TemperatureRange>
    </crela:hasAverageAnnualTemperature>
  </zone:B>
  <zone:B rdf:ID="HotLowLatitudeSteppeClimate"/>

  <zone:B rdf:ID="BSk">
    <owl:sameAs rdf:resource="#ColdMidlatitudeSteppeClimate"/>
    <crela:hasAverageAnnualTemperature>
      <temp:TemperatureRange>
        <mrela:hasUpperBound rdf:datatype="&xsd;integer">18</mrela:hasUpperBound>
      </temp:TemperatureRange>
    </crela:hasAverageAnnualTemperature>
    <rdfs:comment xml:lang="en">The BSk climate classification, also known as cold midlatitude steppe climate classification, is characterized by having mean annual temperatures less than 18 degree C.</rdfs:comment>
  </zone:B>
  <zone:B rdf:ID="ColdMidlatitudeSteppeClimate"/>

  <zone:B rdf:ID="BW">
    <owl:sameAs rdf:resource="#AridClimate"/>
    <owl:sameAs rdf:resource="#Arid"/>
    <rdfs:comment xml:lang="en">The BW climate classification, also known as the arid climate classification, is characterized by having precipitation amounts less than 1/2 potential evapotranspiration (POTET).</rdfs:comment>
        <crela:hasAverageAnnualPrecipitation>
          <thic:PrecipitationRange>
            <srela:hasUpperQuantity rdf:resource="&thic;AnnualHalfPotentialEvapotranspiration"/>
          </thic:PrecipitationRange>
        </crela:hasAverageAnnualPrecipitation>
  </zone:B>
  <zone:B rdf:ID="AridClimate"/>
  <zone:B rdf:ID="Arid"/>

  <zone:B rdf:ID="BWh">
    <owl:sameAs rdf:resource="#HotLowLatitudeDesertClimate"/>
    <rdfs:comment xml:lang="en">the BWh climate classification, also known as the hot low-latitude desert, is characterized by having mean annual temperatures greater than 18 degree C.</rdfs:comment>
    <crela:hasAverageAnnualTemperature>
      <temp:TemperatureRange>
        <mrela:hasLowerBound rdf:datatype="&xsd;integer">18</mrela:hasLowerBound>
      </temp:TemperatureRange>
    </crela:hasAverageAnnualTemperature>
  </zone:B>
  <zone:B rdf:ID="HotLowLatitudeDesertClimate"/>

  <zone:B rdf:ID="BWk">
    <owl:sameAs rdf:resource="#ColdMidlatitudeDesertClimate"/>
    <rdfs:comment xml:lang="en">The BWk climate classification, also known as the cold midlatitude desert, is characterized by having mean annual temperatures less than 18 degree C.</rdfs:comment>
    <crela:hasAverageAnnualTemperature>
      <temp:TemperatureRange>
        <mrela:hasUpperBound rdf:datatype="&xsd;integer">18</mrela:hasUpperBound>
      </temp:TemperatureRange>
    </crela:hasAverageAnnualTemperature>
  </zone:B>
  <zone:B rdf:ID="ColdMidlatitudeDesertClimate"/>

  <zone:C rdf:ID="Cfa">
    <crela:hasAverageWarmestMonthTemperature>
      <temp:TemperatureRange>
        <mrela:hasLowerBound rdf:datatype="&xsd;integer">22</mrela:hasLowerBound>
      </temp:TemperatureRange>
    </crela:hasAverageWarmestMonthTemperature>
    <rdfs:comment xml:lang="en">The Cfa climate classification is characterized by year-round precipitation, hot summers, and having the warmest month above 22 degree C.</rdfs:comment>
  </zone:C>

  <zone:C rdf:ID="Cfb">
    <crela:hasAverageWarmestMonthTemperature>
      <temp:TemperatureRange>
        <mrela:hasUpperBound rdf:datatype="&xsd;integer">22</mrela:hasUpperBound>
      </temp:TemperatureRange>
    </crela:hasAverageWarmestMonthTemperature>
    <crela:hasAverageWinterDuration>
      <ptime:MonthRange>
        <mrela:hasLowerBound rdf:datatype="&xsd;integer">4</mrela:hasLowerBound>
      </ptime:MonthRange>
    </crela:hasAverageWinterDuration>
    <rdfs:comment xml:lang="en">The Cfb climate classfication receives year-round precipitation, its warmest month is below 22 degree C and has 4 months above 10 degree C.</rdfs:comment>
  </zone:C>

  <zone:C rdf:ID="Cfc">
    <crela:hasAverageWinterDuration>
      <ptime:MonthRange>
        <mrela:hasLowerBound rdf:datatype="&xsd;integer">1</mrela:hasLowerBound>
        <mrela:hasUpperBound rdf:datatype="&xsd;integer">3</mrela:hasUpperBound>
      </ptime:MonthRange>
    </crela:hasAverageWinterDuration>
    <rdfs:comment xml:lang="en">The Cfc climate classification is charactericized by year-round precipitation and having 1 - 3 months with temperatures above 10 degree C.</rdfs:comment>
  </zone:C>

  <zone:C rdf:ID="Csa">
    <crela:hasWetSeason rdf:resource="&time;Winter"/>
    <crela:hasDrySeason rdf:resource="&time;Summer"/>
    <crela:hasAverageWarmestMonthTemperature>
      <temp:TemperatureRange>
        <mrela:hasLowerBound rdf:datatype="&xsd;integer">22</mrela:hasLowerBound>
      </temp:TemperatureRange>
    </crela:hasAverageWarmestMonthTemperature>
    <rdfs:comment xml:lang="en">The Csa climate classification is characterized by pronounced summer droughts with 70% of precipitation in the winter and hot summers with its warmest month above 22 degree C.</rdfs:comment>
  </zone:C>

  <zone:C rdf:ID="Csb">
    <rdf:type rdf:resource="#WetSummerDryWinterClimate"/>
    <crela:hasAverageWarmestMonthTemperature>
      <temp:TemperatureRange>
        <mrela:hasLowerBound rdf:datatype="&xsd;integer">10</mrela:hasLowerBound>
        <mrela:hasUpperBound rdf:datatype="&xsd;integer">22</mrela:hasUpperBound>
      </temp:TemperatureRange>
    </crela:hasAverageWarmestMonthTemperature>
  </zone:C>

  <zone:C rdf:ID="Cwa">
    <rdf:type rdf:resource="#WetSummerDryWinterClimate"/>
    <crela:hasAverageWarmestMonthTemperature>
      <temp:TemperatureRange>
        <mrela:hasLowerBound rdf:datatype="&xsd;integer">22</mrela:hasLowerBound>
      </temp:TemperatureRange>
    </crela:hasAverageWarmestMonthTemperature>
    <rdfs:comment xml:lang="en">the Cwa climate classification is characterized by winter drought, summer's wettest month getting 10 times more precipitation than driest winter month, and the warmest month being above 22 degree C.</rdfs:comment>
  </zone:C>

  <zone:D rdf:ID="Dfa">
    <crela:hasAverageWarmestMonthTemperature>
      <temp:TemperatureRange>
        <mrela:hasLowerBound rdf:datatype="&xsd;integer">22</mrela:hasLowerBound>
      </temp:TemperatureRange>
    </crela:hasAverageWarmestMonthTemperature>
    <rdfs:comment xml:lang="en">The Dfa climate classification is characterized by having year-round precipitation and warmest month temperatures above 22 degree C.</rdfs:comment>
  </zone:D>

  <zone:D rdf:ID="Dfb">
    <rdfs:comment xml:lang="en">The Dfb climate classifcation is characterized by having year-round precipitation and warmest month temperatures below 22 degree C.</rdfs:comment>
    <crela:hasAverageWarmestMonthTemperature>
      <temp:TemperatureRange>
        <mrela:hasUpperBound rdf:datatype="&xsd;integer">22</mrela:hasUpperBound>
      </temp:TemperatureRange>
    </crela:hasAverageWarmestMonthTemperature>
  </zone:D>

  <zone:D rdf:ID="Dfc">
    <crela:hasAverageWinterDuration>
      <ptime:MonthRange>
        <mrela:hasLowerBound rdf:datatype="&xsd;integer">1</mrela:hasLowerBound>
        <mrela:hasUpperBound rdf:datatype="&xsd;integer">4</mrela:hasUpperBound>
      </ptime:MonthRange>
    </crela:hasAverageWinterDuration>
    <rdfs:comment xml:lang="en">The Dfc climate classification is characterized by having year-round precipitation and having 1 - 4 months above 10 degree C.</rdfs:comment>
  </zone:D>

  <zone:D rdf:ID="Dwa">
    <rdf:type rdf:resource="#DryWinterClimate"/>
    <crela:hasAverageWarmestMonthTemperature>
      <temp:TemperatureRange>
        <mrela:hasLowerBound rdf:datatype="&xsd;integer">22</mrela:hasLowerBound>
      </temp:TemperatureRange>
    </crela:hasAverageWarmestMonthTemperature>
    <rdfs:comment xml:lang="en">The Dwa climate classification is characterized by winter drought and warmest month temperatures above 22 degree C.</rdfs:comment>
  </zone:D>

  <zone:D rdf:ID="Dwb">
    <rdf:type rdf:resource="#DryWinterClimate"/>
    <crela:hasAverageWarmestMonthTemperature>
      <temp:TemperatureRange>
        <mrela:hasUpperBound rdf:datatype="&xsd;integer">22</mrela:hasUpperBound>
      </temp:TemperatureRange>
    </crela:hasAverageWarmestMonthTemperature>
    <rdfs:comment xml:lang="en">The Dwb climate classification is characterized by winter drought and warmest month temperatures below 22 degree C.</rdfs:comment>
  </zone:D>

  <zone:D rdf:ID="Dwc">
    <rdf:type rdf:resource="#DryWinterClimate"/>
    <rdfs:comment xml:lang="en">The Dwc climate classification is characterized by winter drought and haviong 1 - 4 months with temperatures above 10 degrees C.</rdfs:comment>
    <crela:hasAverageWinterDuration>
      <ptime:MonthRange>
        <mrela:hasLowerBound rdf:datatype="&xsd;integer">1</mrela:hasLowerBound>
        <mrela:hasUpperBound rdf:datatype="&xsd;integer">4</mrela:hasUpperBound>
      </ptime:MonthRange>
    </crela:hasAverageWinterDuration>
  </zone:D>

  <zone:D rdf:ID="Dwd">
    <rdf:type rdf:resource="#DryWinterClimate"/>
    <rdfs:comment xml:lang="en">The Dwd climate classification is characterized by winter drought and having coldest month temperatures below -38 degree C (in Siberia only).</rdfs:comment>
    <crela:hasAverageColdestMonthTemperature>
      <temp:TemperatureRange>
        <mrela:hasUpperBound rdf:datatype="&xsd;integer">-38</mrela:hasUpperBound>
      </temp:TemperatureRange>
    </crela:hasAverageColdestMonthTemperature>
  </zone:D>

  <zone:E rdf:ID="EF">
    <owl:sameAs rdf:resource="#IceCapClimate"/>
    <rdfs:comment xml:lang="en">The EF climate classification, also known as the Ice Cap climate classification, is characterized by having warmest month temperatures below 0 degrees C and having precipitation exceeding very small potential evapotranspiration (POTET).</rdfs:comment>
    <crela:hasAverageWarmestMonthTemperature>
      <temp:TemperatureRange>
        <mrela:hasUpperBound rdf:datatype="&xsd;integer">0</mrela:hasUpperBound>
      </temp:TemperatureRange>
    </crela:hasAverageWarmestMonthTemperature>
        <crela:hasAverageAnnualPrecipitation>
          <thic:PrecipitationRange>
            <srela:hasLowerQuantity rdf:resource="&thic;AnnualPotentialEvapotranspiration"/>
          </thic:PrecipitationRange>
        </crela:hasAverageAnnualPrecipitation>
  </zone:E>
  <zone:E rdf:ID="IceCapClimate"/>

  <zone:E rdf:ID="EM">
    <owl:sameAs rdf:resource="#PolarMarineClimate"/>
    <rdfs:comment xml:lang="en">The EM climate classification, also known as the polar marine climate classification, is characterized by all months having temperatures above -7 degree C, warmest month above 0 degree C, and annual temperatures less than 17 degree C.</rdfs:comment>
    <crela:hasAverageMonthlyTemperature>
      <temp:TemperatureRange>
        <mrela:hasLowerBound rdf:datatype="&xsd;integer">-7</mrela:hasLowerBound>
      </temp:TemperatureRange>
    </crela:hasAverageMonthlyTemperature>
    <crela:hasAverageWarmestMonthTemperature>
      <temp:TemperatureRange>
        <mrela:hasLowerBound rdf:datatype="&xsd;integer">0</mrela:hasLowerBound>
      </temp:TemperatureRange>
    </crela:hasAverageWarmestMonthTemperature>
    <crela:hasAverageAnnualTemperature>
      <temp:TemperatureRange>
        <mrela:hasUpperBound rdf:datatype="&xsd;integer">17</mrela:hasUpperBound>
      </temp:TemperatureRange>
    </crela:hasAverageAnnualTemperature>
  </zone:E>
  <zone:E rdf:ID="PolarMarineClimate"/>

  <zone:E rdf:ID="ET">
    <owl:sameAs rdf:resource="#TundraClimate"/>
    <crela:hasAverageSnowCoverDuration>
      <ptime:MonthRange>
        <mrela:hasLowerBound rdf:datatype="&xsd;integer">8</mrela:hasLowerBound>
        <mrela:hasUpperBound rdf:datatype="&xsd;integer">10</mrela:hasUpperBound>
      </ptime:MonthRange>
    </crela:hasAverageSnowCoverDuration>
    <crela:hasWarmestMonthTemperature>
      <temp:TemperatureRange>
        <mrela:hasLowerBound rdf:datatype="&xsd;integer">0</mrela:hasLowerBound>
        <mrela:hasUpperBound rdf:datatype="&xsd;integer">10</mrela:hasUpperBound>
      </temp:TemperatureRange>
    </crela:hasWarmestMonthTemperature>
    <crela:hasAverageAnnualPrecipitation>
      <thic:PrecipitationRange>
        <srela:hasLowerQuantity rdf:resource="&thic;AnnualPotentialEvapotranspiration"/>
      </thic:PrecipitationRange>
    </crela:hasAverageAnnualPrecipitation>
    <rdfs:comment xml:lang="en">The ET climate classification, also known as the tundra climate classification, is characterizex by warmest month temperatures between 0 - 10 degree C, precipitation exceeds small potential evapotranspiration demand, and has snow cover 8 - 10 months out of the year.</rdfs:comment>
  </zone:E>
  <zone:E rdf:ID="TundraClimate"/>

  <owl:Class rdf:about="#Equator">
    <rdfs:subClassOf rdf:resource="#TropicalClimateZone" />
  </owl:Class>

</rdf:RDF>
