<?xml version="1.0" encoding="UTF-8"?>

<!DOCTYPE rdf:RDF [
  <!ENTITY petr "http://sweet.jpl.nasa.gov/2.3/matrRock.owl">
  <!ENTITY screla "http://sweet.jpl.nasa.gov/2.3/relaSci.owl">
  <!ENTITY srela "http://sweet.jpl.nasa.gov/2.3/relaSpace.owl">
  <!ENTITY prela "http://sweet.jpl.nasa.gov/2.3/relaPhysical.owl">
  <!ENTITY rela "http://sweet.jpl.nasa.gov/2.3/rela.owl">
  <!ENTITY prop "http://sweet.jpl.nasa.gov/2.3/propSpace.owl">
  <!ENTITY geol "http://sweet.jpl.nasa.gov/2.3/realmGeol.owl">
  <!ENTITY planet "http://sweet.jpl.nasa.gov/2.3/realm.owl">
  <!ENTITY owl "http://www.w3.org/2002/07/owl#">
  <!ENTITY rdf "http://www.w3.org/1999/02/22-rdf-syntax-ns#">
  <!ENTITY rdfs "http://www.w3.org/2000/01/rdf-schema#">
  <!ENTITY xsd "http://www.w3.org/2001/XMLSchema#">
]>

<rdf:RDF xml:base="&geol;"
         xmlns:prop="&prop;"
         xmlns:screla="&screla;"
         xmlns:srela="&srela;"
         xmlns:prela="&prela;"
         xmlns:rela="&rela;"
         xmlns:planet="&planet;"
         xmlns:petr="&petr;"
         xmlns:geol="&geol;"
         xmlns:owl="&owl;"
         xmlns:rdf="&rdf;"
         xmlns:rdfs="&rdfs;"
 	 xmlns:xsd="&xsd;">

<!-- Ontology Information -->
  <owl:Ontology rdf:about="" owl:versionInfo="2.3">
     <rdfs:label>SWEET Ontology</rdfs:label>
     <owl:imports rdf:resource="&petr;"/>
     <owl:imports rdf:resource="&prop;"/>
     <owl:imports rdf:resource="&screla;"/>
     <owl:imports rdf:resource="&srela;"/>
     <owl:imports rdf:resource="&prela;"/>
     <owl:imports rdf:resource="&rela;"/>
     <owl:imports rdf:resource="&planet;"/>
  </owl:Ontology>

<!-- Realms -->

  <owl:Class rdf:ID="Bedrock">
    <rdfs:subClassOf rdf:resource="#GeosphereLayer"/>
  </owl:Class>

  <owl:Class rdf:about="#Continental">
    <rdfs:subClassOf rdf:resource="&planet;#PlanetaryRealm"/>
  </owl:Class>

  <owl:Class rdf:ID="Core">
    <rdfs:subClassOf rdf:resource="#GeosphereLayer"/>
    <rdfs:comment xml:lang="en">The central most structure inside the earth. The core does not allow shear waves to pass through it, while the speed of travel (seismic velocity) is different in the other layers. [Wikipedia]</rdfs:comment>
  </owl:Class>

  <owl:Class rdf:ID="Crust">
    <rdfs:subClassOf rdf:resource="#GeosphereLayer"/>
     <rdfs:subClassOf>
      <owl:Restriction>
        <owl:onProperty rdf:resource="&srela;#hasLowerBoundary"/>
        <owl:allValuesFrom rdf:resource="#Moho"/>
      </owl:Restriction>
     </rdfs:subClassOf>
    <rdfs:comment xml:lang="en">The crust is the outermost solid shell of a rocky planet or moon, which is chemically distinct from the underlying mantle.  [Wikipedia]</rdfs:comment>
  </owl:Class>

  <owl:Class rdf:ID="BrittleDuctileTransitionZone">
    <rdfs:subClassOf rdf:resource="#Crust"/>
    <rdfs:comment xml:lang="en">D" layer is the layer which separates the mantle from the core. D_ may consist of material from subducted slabs that descended and came to rest at the core-mantle boundary and/or from a new mineral polymorph discovered in perovskite called post-perovskite.[Wikipedia]</rdfs:comment>
  </owl:Class>

  <owl:Class rdf:ID="DLayer">
    <rdfs:subClassOf rdf:resource="#Mantle"/>
    <rdfs:comment xml:lang="en">D" layer is the layer which separates the mantle from the core. D_ may consist of material from subducted slabs that descended and came to rest at the core-mantle boundary and/or from a new mineral polymorph discovered in perovskite called post-perovskite.[Wikipedia]</rdfs:comment>
  </owl:Class>

  <owl:Class rdf:ID="Fabric">
    <rdfs:subClassOf rdf:resource="&prop;#Configuration"/>
  </owl:Class>

  <owl:Class rdf:about="#GeologicFeature">
    <rdfs:subClassOf rdf:resource="&planet;#PlanetaryRealm"/>
    <rdfs:subClassOf>
      <owl:Restriction>
        <owl:allValuesFrom rdf:resource="&planet;#Geosphere"/>
        <owl:onProperty rdf:resource="&rela;#hasRealm"/>
      </owl:Restriction>
    </rdfs:subClassOf>
    <rdfs:comment xml:lang="en"> or Surface Feature is a distinct recognizable structure within a larger context such as a stream bed, fissure, dike, etc.</rdfs:comment>
  </owl:Class>

  <owl:Class rdf:ID="GeosphereLayer">
    <rdfs:subClassOf rdf:resource="&planet;#PlanetaryLayer"/>
    <rdfs:subClassOf rdf:resource="#Subsurface"/>
    <rdfs:subClassOf>
      <owl:Restriction>
        <owl:onProperty rdf:resource="&rela;#hasRealm"/>
        <owl:allValuesFrom rdf:resource="&planet;#Geosphere"/>
      </owl:Restriction>
    </rdfs:subClassOf>
  </owl:Class>

  <owl:Class rdf:about="#GeologicProvince">
    <rdfs:subClassOf rdf:resource="#GeologicFeature"/>
    <rdfs:comment xml:lang="en"> A geologic or geomorphic province is a spatial entity with common geologic/geomorphic attributes. A province may include a single dominant structural element such as a basin or a fold belt, or a number of contiguous related elements. Most commonly, provinces are classified by age, origin, or mineral resource.    [Wikipedia]</rdfs:comment>
  </owl:Class>

  <owl:Class rdf:about="#GeologicStructure">
    <rdfs:subClassOf rdf:resource="&planet;#Geosphere"/>
    <rdfs:subClassOf>
      <owl:Restriction>
        <owl:onProperty rdf:resource="&rela;#hasRealm"/>
        <owl:allValuesFrom rdf:resource="&planet;#Geosphere"/>
      </owl:Restriction>
    </rdfs:subClassOf>
  </owl:Class>

  <owl:Class rdf:ID="InnerCore">
    <rdfs:subClassOf rdf:resource="#Mantle"/>
    <owl:disjointWith rdf:resource="#OuterCore" />
    <rdfs:comment xml:lang="en">The solid inner core was discovered in 1936 by Inge Lehmann and is generally believed to be composed primarily of iron and some nickel.[Wikipedia]</rdfs:comment>
  </owl:Class>

  <owl:Class rdf:ID="Lithosphere">
    <rdfs:subClassOf rdf:resource="#GeosphereLayer"/>
    <rdfs:subClassOf>
      <owl:Restriction>
        <owl:onProperty rdf:resource="&screla;#containsMaterial"/>
        <owl:allValuesFrom rdf:resource="&petr;#Rock"/>
      </owl:Restriction>
    </rdfs:subClassOf>
    <rdfs:comment xml:lang="en">In the Earth, the lithosphere includes the crust and the uppermost mantle, which constitute the hard and rigid outer layer of the planet. The division of Earth's outer layers into lithosphere and asthenosphere should not be confused with the chemical subdivision of the outer Earth into mantle, and crust. All crust is in the lithosphere, but lithosphere generally contains more mantle than crust. [Wikipedia]</rdfs:comment>
  </owl:Class>

  <owl:Class rdf:ID="LowerMantle">
    <rdfs:subClassOf rdf:resource="#Mantle"/>
    <rdfs:comment xml:lang="en">Very little is known about the lower mantle apart from that it appears to be relatively seismically homogeneous. The lower mantle is under tremendous pressure and therefore has a higher viscosity than the upper mantle.[Wikipedia]</rdfs:comment>
  </owl:Class>

  <owl:Class rdf:ID="Mantle">
    <rdfs:subClassOf rdf:resource="#GeosphereLayer"/>
     <rdfs:subClassOf>
      <owl:Restriction>
        <owl:onProperty rdf:resource="&srela;#hasUpperBoundary"/>
        <owl:allValuesFrom rdf:resource="#Moho"/>
      </owl:Restriction>
     </rdfs:subClassOf>
    <rdfs:comment xml:lang="en">The mantle is a highly viscous layer between the crust and the outer core. Earth's mantle is an approximately 2,970 km thick (~1,800 mi) rocky shell that constitutes approximately 84 percent of Earth's volume.  [Wikipedia]</rdfs:comment>
  </owl:Class>

  <owl:Class rdf:ID="Mesosphere">
    <owl:equivalentClass rdf:resource="#UpperMantleRigid"/>
    <rdfs:comment xml:lang="en">The mesosphere refers to the mantle in the region between the asthenosphere and the outer core. The upper boundary is defined as the sharp increase in seismic wave velocities and density at a depth of 660 km. [Wikipedia]</rdfs:comment>
  </owl:Class>

  <owl:Class rdf:ID="OuterCore">
    <rdfs:subClassOf rdf:resource="#Mantle"/>
    <rdfs:comment xml:lang="en">The liquid outer core surrounds the inner core and is believed to be composed of iron mixed with nickel and trace amounts of lighter elements. [Wikipedia]</rdfs:comment>
  </owl:Class>

  <owl:Class rdf:about="#SolidEarth">
    <owl:equivalentClass rdf:resource="&planet;#Geosphere"/>
  </owl:Class>

  <owl:Class rdf:about="#SkinLayer">
    <owl:equivalentClass rdf:resource="#Crust"/>
  </owl:Class>

  <owl:Class rdf:about="#TransitionalCrust">
    <rdfs:subClassOf rdf:resource="#Crust"/>
    <rdfs:comment xml:lang="en">Transitional crust is crust that is thinned by the upwelling of mantle.  [Wikipedia]</rdfs:comment>
  </owl:Class>

  <owl:Class rdf:about="#TransitionalLithosphere">
    <rdfs:subClassOf rdf:resource="#GeosphereLayer"/>
    <rdfs:subClassOf>
      <owl:Restriction>
        <owl:someValuesFrom rdf:resource="#TransitionalCrust"/>
        <owl:onProperty rdf:resource="&prela;#hasPlanetaryStructure"/>
      </owl:Restriction>
    </rdfs:subClassOf>
  </owl:Class>

  <owl:Class rdf:about="#Asthenosphere">
    <rdfs:subClassOf rdf:resource="#UpperMantle"/>
    <owl:equivalentClass rdf:resource="#UpperMantleFlowing"/>
    <rdfs:comment xml:lang="en">The asthenosphere is a portion of the upper mantle just below the lithosphere.  Seismic waves pass relatively slowly through the asthenosphere, compared to the overlying lithospheric mantle, thus it has been called the low-velocity zone. [Wikipedia]</rdfs:comment>
  </owl:Class>
  <owl:Class rdf:ID="UpperMantleFlowing"/>

  <owl:Class rdf:about="#UpperMantleRigid">
    <rdfs:subClassOf rdf:resource="#UpperMantle"/>
    <rdfs:comment xml:lang="en">The uppermost mantle plus overlying crust are relatively rigid and form the lithosphere, an irregular layer with a maximum thickness of perhaps 200 km. [Wikipedia]</rdfs:comment>
  </owl:Class>

  <owl:Class rdf:about="#UpperMantle">
    <rdfs:subClassOf rdf:resource="#Mantle"/>
    <rdfs:comment xml:lang="en">The mantle is divided into sections based upon results from seismology. The upper mantle is the region from 33â€“410 km (20 to 254 miles). The upper part of the mantle is composed mostly of peridotite, a rock denser than rocks common in the overlying crust. [Wikipedia]</rdfs:comment>
  </owl:Class>

  <owl:Class rdf:about="#Basement">
    <rdfs:subClassOf rdf:resource="#GeologicStructure"/>
  </owl:Class>

  <owl:Class rdf:about="#Cover">
    <rdfs:subClassOf rdf:resource="#GeologicStructure"/>
  </owl:Class>


<!-- Realms -->
  <owl:Class rdf:about="#Batholith">
    <rdfs:subClassOf rdf:resource="#PlutonicStructure"/>
    <rdfs:comment xml:lang="en">A batholith is a large emplacement of igneous intrusive (also called plutonic) rock that forms from cooled magma deep in the Earth's crust. Batholiths are almost always made mostly of felsic or intermediate rock-types, such as granite, quartz monzonite, or diorite (see also granite dome).There is also an important geographic usage of the term batholith. For a geographer, a batholith is an exposed area of mostly continuous plutonic rock that covers an area larger than 100 square kilometers. [Wikipedia]</rdfs:comment>
  </owl:Class>

  <owl:Class rdf:about="#Dike">
    <rdfs:subClassOf rdf:resource="#PlutonicStructure"/>
    <rdfs:comment xml:lang="en">Dikes, long, planar (sheet) igneous intrusions, enter along cracks, and therefore often form in large numbers in areas that are being actively deformed. [Wikipedia]</rdfs:comment>
  </owl:Class>

  <owl:Class rdf:about="#GiantDikeSwarm">
    <rdfs:subClassOf rdf:resource="#Dike"/>
    <rdfs:comment xml:lang="en">A dike swarm or dyke swarm in geology is a major group of parallel, linear, or radially oriented dikes intruded within continental crust. [Wikipedia]</rdfs:comment>
  </owl:Class>

  <owl:Class rdf:about="#Laccolith">
    <rdfs:subClassOf rdf:resource="#PlutonicStructure"/>
    <rdfs:comment xml:lang="en"> [Pluton] Igneous intrusion - A laccolith is an igneous intrusion (or concordant pluton) that has been injected between two layers of sedimentary rock. The pressure of the magma is high enough that the overlying strata are forced upward, giving the laccolith a dome or mushroom-like form with a generally planar base.Laccoliths tend to form at relatively shallow depths and are typically formed by relatively viscous magmas, such as those that crystallize to diorite, granodiorite, and granite.[Wikipedia]</rdfs:comment>
  </owl:Class>

  <owl:Class rdf:about="#Lopolith">
    <rdfs:subClassOf rdf:resource="#PlutonicStructure"/>
    <rdfs:comment xml:lang="en">[Pluton] Igneous intrusion - A lopolith is a large igneous intrusion which is lenticular in shape with a depressed central region. Lopoliths are generally concordant with the intruded strata with dike or funnel-shaped feeder bodies below the body. Lopoliths typically consist of large ultramafic to mafic layered intrusions that range in age from Archean to Eocene. [Wikipedia]</rdfs:comment>
  </owl:Class>

  <owl:Class rdf:about="#Sill">
    <rdfs:subClassOf rdf:resource="#PlutonicStructure"/>
    <rdfs:comment xml:lang="en">[Pluton] Igneous intrusion - A sill is a tabular pluton that has intruded between older layers of sedimentary rock, beds of volcanic lava or tuff, or even along the direction of foliation in metamorphic rock. The term sill is synonymous with concordant intrusive sheet. This means that the sill does not cut across preexisting rocks, in contrast to dikes, which do cut across older rocks. [Wikipedia]</rdfs:comment>
  </owl:Class>

  <owl:Class rdf:about="#PlutonicStructure">
    <rdfs:subClassOf rdf:resource="&geol;#GeologicStructure"/>
  </owl:Class>

  <owl:Class rdf:about="#SeismicZone">
    <rdfs:subClassOf rdf:resource="&geol;#GeologicFeature"/>
    <rdfs:comment xml:lang="en">Seismic Zones are broad elongated regions along a fault line where earthquakes take place. [Wikipedia]</rdfs:comment>
  </owl:Class>
  
  <owl:Class rdf:ID="GuttenburgDiscontinuity">
    <rdfs:subClassOf rdf:resource="#GeologicBoundary"/>
    <owl:equivalentClass rdf:resource="#CoreMantleBoundary"/>
    <rdfs:comment xml:lang="en">The core-mantle boundary. This discontinuity is due to the differences between the acoustic impedances of the solid mantle and the molten outer core. P-wave velocities are much slower in the outer core than in the deep mantle while S-waves do not exist at all in the liquid portion of the core. Corresponds to top of D"". [Wikipedia]</rdfs:comment>
  </owl:Class>
  <owl:Class rdf:ID="CoreMantleBoundary"/>

  <owl:Class rdf:ID="LehmannDiscontinuity">
    <rdfs:subClassOf rdf:resource="#GeologicBoundary"/>
    <rdfs:comment xml:lang="en">Boundary between Asthenosphere and Lithosphere. It is the discontinuity in seismic velocity near a depth of 220 km. It appears beneath continents, but not usually beneath oceans, and does not readily appear in globally-averaged studies [Wikipedia]</rdfs:comment>
  </owl:Class>

  <owl:Class rdf:ID="Moho">
    <rdfs:subClassOf rdf:resource="#GeologicBoundary"/>
    <owl:equivalentClass rdf:resource="#Mohorovi_i_Discontinuity"/>
    <owl:equivalentClass rdf:resource="#CrustMantleBoundary"/>
    <rdfs:comment xml:lang="en">The boundary between the crust and mantle is conventionally placed at the Mohorovi_i_ discontinuity, a boundary defined by a contrast in seismic velocity. [Wikipedia]</rdfs:comment>
  </owl:Class>
  <owl:Class rdf:ID="Mohorovi_i_Discontinuity"/>
  <owl:Class rdf:ID="CrustMantleBoundary"/>

  <owl:Class rdf:about="#GeologicBoundary">
    <rdfs:subClassOf rdf:resource="&planet;#PlanetaryBoundary"/>
  </owl:Class>

  <owl:Class rdf:about="#Subsurface">
    <rdfs:subClassOf rdf:resource="&planet;#PlanetaryRealm"/>
    <owl:disjointWith rdf:resource="&planet;#PlanetarySurface" />
  </owl:Class>

</rdf:RDF>
