<?xml version="1.0" encoding="UTF-8"?>

<!DOCTYPE rdf:RDF [
  <!ENTITY land "http://sweet.jpl.nasa.gov/2.3/realmLandform.owl">
  <!ENTITY glac "http://sweet.jpl.nasa.gov/2.3/realmLandGlacial.owl">
  <!ENTITY owl "http://www.w3.org/2002/07/owl#">
  <!ENTITY rdf "http://www.w3.org/1999/02/22-rdf-syntax-ns#">
  <!ENTITY rdfs "http://www.w3.org/2000/01/rdf-schema#">
  <!ENTITY xsd "http://www.w3.org/2001/XMLSchema#">
]>

<rdf:RDF xml:base="&glac;"
         xmlns:owl="&owl;"
         xmlns:rdf="&rdf;"
         xmlns:rdfs="&rdfs;"
         xmlns:xsd="&xsd;"
         xmlns:land="&land;"
         xmlns:glac="&glac;"
>
<!-- Ontology Information -->
  <owl:Ontology rdf:about=""
                owl:versionInfo="2.3">
     <rdfs:label>SWEET Ontology</rdfs:label>
     <owl:imports rdf:resource="&land;"/>
  </owl:Ontology>

  <owl:Class rdf:about="#GlacialLandform">
    <rdfs:subClassOf rdf:resource="&land;#Landform"/>
  </owl:Class>

  <owl:Class rdf:about="#Arete">
    <rdfs:subClassOf rdf:resource="#GlacialPlain"/>
    <rdfs:comment xml:lang="en">A thin, almost knife-like, ridge of rock which is typically formed when two glaciers erode parallel U-shaped valleys.</rdfs:comment> 
  </owl:Class>

  <owl:Class rdf:about="#Cirque">
    <rdfs:subClassOf rdf:resource="#GlacialPlain"/>
    <rdfs:comment xml:lang="en">An amphitheatre-like valley head, formed at the head of a valley glacier by erosion.</rdfs:comment> 
  </owl:Class>

  <owl:Class rdf:about="#Esker">
    <rdfs:subClassOf rdf:resource="#GlacialLandform"/>
    <rdfs:comment xml:lang="en">A long winding ridge of stratified sand and gravel, examples of which occur in glaciated and formerly glaciated regions.</rdfs:comment> 
  </owl:Class>

  <owl:Class rdf:about="#GlacialPlain">
    <rdfs:subClassOf rdf:resource="&land;#Plain"/>
    <rdfs:subClassOf rdf:resource="#GlacialLandform"/>
  </owl:Class>

  <owl:Class rdf:about="#GlacialOutwashPlain">
    <rdfs:subClassOf rdf:resource="#GlacialPlain"/>
  </owl:Class>

  <owl:Class rdf:about="#Kame">
    <rdfs:subClassOf rdf:resource="#GlacialLandform"/>
    <rdfs:comment xml:lang="en">An irregularly shaped hill or mound composed of sand, gravel and till that accumulates in a depresson on a retreating glacier, and is then deposited with further melting.[Wikipedia]</rdfs:comment> 
  </owl:Class>

  <owl:Class rdf:about="#Moraine">
    <rdfs:subClassOf rdf:resource="#GlacialPlain"/>
    <owl:equivalentClass rdf:resource="#GlacialMoraine"/>
    <rdfs:comment xml:lang="en">Any glacially formed accumulation of unconsolidated glacial debris (soil and rock) which can occur in currently glaciated and formerly glaciated regions.</rdfs:comment> 
  </owl:Class>
  <owl:Class rdf:about="#GlacialMoraine"/>

  <owl:Class rdf:about="#OutwashFan">
    <rdfs:subClassOf rdf:resource="#GlacialLandform"/>
    <rdfs:comment xml:lang="en">A fan-shaped body of sediments deposited by braided streams from a melting glacier. Sediment locked within the ice of the glacier gets transported by the streams of meltwater and deposits on the outwash plain at the terminus of the glacier.</rdfs:comment> 
  </owl:Class>

  <owl:Class rdf:ID="RockGlacier">
    <rdfs:subClassOf rdf:resource="#GlacialLandform"/>
    <rdfs:comment xml:lang="en">Rock glaciers are distinctive geomorphological landforms of blocky detritus which may extend outward and downslope from talus cones or from glaciers or the terminal moraines of glaciers. [Wikipedia]</rdfs:comment>
  </owl:Class>
  
  <owl:Class rdf:about="#Sandur">
    <rdfs:subClassOf rdf:resource="#GlacialOutwashPlain"/>
    <rdfs:comment xml:lang="en">A glacial outwash plain formed of sediments deposited by meltwater at the terminus of a glacier.</rdfs:comment>
  </owl:Class>

  <owl:Class rdf:about="#TillPlain">
    <rdfs:subClassOf rdf:resource="#GlacialPlain"/>
    <owl:equivalentClass rdf:resource="#Till"/>
    <rdfs:comment xml:lang="en">An extensive flat plain of glacial till that forms when a sheet of ice becomes detached from the main body of a glacier and melts in place depositing the sediments it carried.</rdfs:comment>
  </owl:Class>
  <owl:Class rdf:about="#Till"/>

  <owl:Class rdf:about="#Thermokarst">
    <rdfs:subClassOf rdf:resource="#GlacialLandform"/>
    <rdfs:comment xml:lang="en">A land surface characterised by very irregular surfaces of marshy hollows and small hummocks formed as ice-rich permafrost thaws.</rdfs:comment>
  </owl:Class>

  <owl:Class rdf:about="#UShapedValley">
    <rdfs:subClassOf rdf:resource="#GlacialLandform"/>
  </owl:Class>

</rdf:RDF>
