<?xml version='1.0' encoding='utf-8'?>
<!--
     Copyright (C)2004 W3C(R) (MIT, ERCIM, Keio), All Rights Reserved.
     W3C viability, trademark, document use and software licensing rules
     apply.                                                             
     http://www.w3.org/Consortium/Legal/
                                        
     This document is governed by the W3C Software License [1] as
     described in the FAQ [2].

     [1] http://www.w3.org/Consortium/Legal/copyright-software-20021231
     [2] http://www.w3.org/Consortium/Legal/IPR-FAQ-20000620.html#DTD
-->
<!DOCTYPE uridef[
  <!ENTITY owl "http://www.w3.org/2002/07/owl">
  <!ENTITY rdf "http://www.w3.org/1999/02/22-rdf-syntax-ns">
  <!ENTITY rdfs "http://www.w3.org/2000/01/rdf-schema">
  <!ENTITY xsd "http://www.w3.org/2001/XMLSchema">
  <!ENTITY ServiceModel "http://www.w3.org/2004/02/wsa/ServiceModel.owl">
  <!ENTITY PolicyModel "http://www.w3.org/2004/02/wsa/PolicyModel.owl">
  <!ENTITY Extensions "http://www.w3.org/2004/02/wsa/Extensions.owl">

]>

<rdf:RDF
  xmlns:owl  ="http://www.w3.org/2002/07/owl#"
  xmlns:rdf  ="http://www.w3.org/1999/02/22-rdf-syntax-ns#"
  xmlns:rdfs ="http://www.w3.org/2000/01/rdf-schema#"
  xmlns:xsd  ="http://www.w3.org/2001/XMLSchema#"
      xml:base	 ="http://www.w3.org/2004/02/wsa/ResourceModel.owl"

  xmlns      ="http://www.w3.org/2004/02/wsa/ResourceModel.owl#"
 >

<owl:Ontology rdf:about="">
 <owl:versionInfo>$Id: ResourceModel.owl,v 1.2 2004/02/05 16:18:21 hugo Exp $</owl:versionInfo>
 <rdfs:comment> Compiled by Massimo Paolucci, Naveen Srinivasan and Katia Sycara. Carnegie Mellon University
 </rdfs:comment>

 <owl:imports rdf:resource="http://www.w3.org/2004/02/wsa/ServiceModel.owl"/>
 <owl:imports rdf:resource="http://www.w3.org/2004/02/wsa/MessageModel.owl"/>
  <owl:imports rdf:resource="http://www.w3.org/2004/02/wsa/PolicyModel.owl"/>
  <owl:imports rdf:resource="http://www.w3.org/2004/02/wsa/Extensions.owl"/>


</owl:Ontology>

<!-- Created: Mon Jan 26 12:49:24 2004 -->

<!-- 2.3.3.1 Discovery -->

<owl:Class rdf:ID="Discovery">
  <rdfs:comment>Discovery is the act of locating a machine-processable description of a Web service-related resource that may have been previously unknown and that meets certain functional criteria. It involves matching a set of functional and other criteria with a set of resource descriptions. The goal is to find an appropriate Web service-related resource
  </rdfs:comment>
  <rdfs:label>Discovery</rdfs:label>
</owl:Class>



<!-- Not Expressed : Discovery involves matching a set of functional and other criteria with a set of resource descriptions.-->

<owl:ObjectProperty rdf:ID="performed_by">
  <rdfs:label>performed_by</rdfs:label>
  <rdfs:comment>
    Discovery may be performed by an agent, or by an end-user
  </rdfs:comment>
  <rdfs:domain rdf:resource="#Discovery"/>
  <rdfs:range rdf:resource="&ServiceModel;#Agent"/>
</owl:ObjectProperty>


<owl:ObjectProperty rdf:ID="discovery_realized_by">
  <rdfs:label>realized_by</rdfs:label>
  <rdfs:comment>
    Discovery may be realized using a discovery service
  </rdfs:comment>
  <rdfs:domain rdf:resource="#Discovery"/>
  <rdfs:range rdf:resource="#Discovery_Service"/>
</owl:ObjectProperty>

<!-- 2.3.3.2 Discovery Service-->



<owl:Class rdf:ID="Discovery_Service">
  <rdfs:label>Discovery_Service</rdfs:label>
  <rdfs:comment>A discovery service is a service that enables agents to retrieve Web service-related resource descriptions
  </rdfs:comment>
  <rdfs:subClassOf rdf:resource="&ServiceModel;#Service"/>
  <rdfs:comment>
    A discovery service is a service
  </rdfs:comment>
</owl:Class>


<owl:ObjectProperty rdf:ID="publish">
  <rdfs:label>publish</rdfs:label>
  <rdfs:comment>A discovery service is used to publish descriptions
  </rdfs:comment>
  <rdfs:domain rdf:resource="#Discovery_Service"/>
  <rdfs:range rdf:resource="#Resource_Description"/>
</owl:ObjectProperty>

<owl:ObjectProperty rdf:ID="search">
  <rdfs:label>search</rdfs:label>
  <rdfs:comment>
    A discovery service is used to search for resources 
  </rdfs:comment>
  <rdfs:domain rdf:resource="#Discovery_Service"/>
  <rdfs:range rdf:resource="#Resource_Description"/>
</owl:ObjectProperty>


<owl:ObjectProperty rdf:ID="used_by">
  <rdfs:label>used by</rdfs:label>
  <rdfs:comment>
    A discovery service may be used by an agent
  </rdfs:comment>
  <rdfs:domain rdf:resource="#Discovery_Service"/>
  <rdfs:range rdf:resource="&ServiceModel;#Agent"/>
</owl:ObjectProperty>

<!-- 2.3.3.3 Identifier-->


<owl:Class rdf:ID="Identifier">
  <rdfs:label>Identifier</rdfs:label>
  <rdfs:comment>
    An identifier is an opaque string of bits that may be used to
    associate with a resource.
  </rdfs:comment>
</owl:Class>

<owl:DatatypeProperty rdf:ID="realized_by">
  <rdfs:label>realized_by</rdfs:label>
  <rdfs:comment>
    an identifier should be realized a URI
  </rdfs:comment>
  <rdfs:domain rdf:resource="#Identifier"/>
  <rdfs:range rdf:resource="&xsd;#uriReference"/>
</owl:DatatypeProperty>

<owl:ObjectProperty rdf:ID="identify">
  <rdfs:label>identify</rdfs:label>
  <rdfs:comment>an identifier identifies a resource that is relevant to the architecture
  </rdfs:comment>
  <rdfs:domain rdf:resource="#Identifier"/>
  <rdfs:range rdf:resource="#Resource"/>
</owl:ObjectProperty>

<!-- 2.3.3.4 Representation -->

<owl:Class rdf:ID="Representation">
  <rdfs:label>Representation</rdfs:label>
  <rdfs:comment>A representation is a piece of data that describes a resource state. 
  </rdfs:comment>
</owl:Class>

<owl:ObjectProperty rdf:ID="representation">
  <rdfs:label>representation</rdfs:label>
  <rdfs:comment>
    a resource may have a representation
  </rdfs:comment>
  <rdfs:domain rdf:resource="#Representation"/>
  <rdfs:range rdf:resource="#Resource"/>
</owl:ObjectProperty>


<!-- 2.3.3.5 Resource-->

<owl:Class rdf:ID="Resource">
  <rdfs:label>Resource</rdfs:label>
  <rdfs:comment>A resource is defined by [RFC 2396] to be anything that can have an identifier. Although resources in general can be anything, this architecture is only concerned with those resources that are relevant to Web services and therefore have some additional characteristics. In particular, they incorporate the concepts of ownership and control: a resource that appears in this architecture is a thing that has a name, may have reasonable representations and which can be said to be owned. The ownership of a resource is critically connected with the right to set policy on the resource.
  </rdfs:comment>
</owl:Class>


<owl:ObjectProperty rdf:ID="identifier">
  <rdfs:label>identifier</rdfs:label>
  <rdfs:comment>
    a resource has an identifier
  </rdfs:comment>
  <owl:inverseOf rdf:resource="#identify"/>
</owl:ObjectProperty>


<owl:ObjectProperty rdf:ID="represented_by">
  <rdfs:label>representation</rdfs:label>
  <rdfs:comment>
    a resource may have zero or more representations
  </rdfs:comment>
  <owl:inverseOf rdf:resource="#representation"/>
</owl:ObjectProperty>


<owl:ObjectProperty rdf:ID="resource_description">
  <rdfs:label>representation</rdfs:label>
  <rdfs:comment>
    a resource may have zero or more resource description  
  </rdfs:comment>
  <rdfs:domain rdf:resource="#Resource"/>
  <rdfs:range rdf:resource="#Resource_Description"/>
</owl:ObjectProperty>


<owl:ObjectProperty rdf:ID="owned_by">
  <rdfs:label>owned_by</rdfs:label>
  <rdfs:comment>
    a resource is owned by a person or an organization 
  </rdfs:comment>
  <rdfs:domain rdf:resource="#Resource"/>
  <rdfs:range rdf:resource="&PolicyModel;#Person_or_Organization"/>
</owl:ObjectProperty>


<owl:ObjectProperty rdf:ID="governed_by">
  <rdfs:label>governed_by</rdfs:label>
  <rdfs:comment>
    a resource may be governed by zero or more policies 
  </rdfs:comment>
  <rdfs:domain rdf:resource="#Resource"/>
  <rdfs:range rdf:resource="&PolicyModel;#Policy"/>
</owl:ObjectProperty>

<!-- 2.3.3.6 Resource description-->


<owl:Class rdf:ID="Resource_Description">
  <rdfs:label>Resource_Description</rdfs:label>
  <rdfs:comment>
    A resource description is any machine readable structure that may
    permit resources to be discovered. Resource descriptions may be of
    many different forms, tailored for specific purposes, but all
    resource descriptions must contain the resource's identifier. (2.3.3.6.1)
  </rdfs:comment>
</owl:Class>

<!-- 
Not Expressed "A resource description contains the resource's identifier Used concept Identifier instead of defining Resource_Identifier"falls in the same category as the MetaProperty Problem described in ServiceModel.owl .

-->

 
<!-- 
Not Expressed " A resource description may reference the policies applicable to the resource" falls in the same category as the MetaProperty Problem described in ServiceModel.owl .

-->

<!-- 
Not Expressed  : We cannot model "A resource description may reference the semantics applicable to the resource" falls in the same category as the MetaProperty Problem described in ServiceModel.owl .

-->

</rdf:RDF>


